src/tactics/FStar.Tactics.V2.Basic.fsti
@@ -132,6 +132,7 @@ val refl_core_check_term              : env -> term -> typ -> tot_or_ghost -> ta
 val refl_tc_term                      : env -> term -> tot_or_ghost -> tac (option (term & typ) & issues)
 val refl_universe_of                  : env -> term -> tac (option universe & issues)
 val refl_check_prop_validity          : env -> term -> tac (option unit & issues)
+val refl_check_type_erasable          : env -> typ -> tac (option unit & issues)
 val refl_check_match_complete         : env -> term -> term -> list pattern -> tac (option (list pattern & list (list RD.binding)))
 val refl_instantiate_implicits        : env -> term -> tac (option (term & typ) & issues)
 val refl_maybe_relate_after_unfolding : env -> term -> term -> tac (option Core.side & issues)
