src/tactics/FStar.Tactics.V2.Interpreter.fst
@@ -631,6 +631,10 @@ let () =
         refl_check_prop_validity RE.e_env RE.e_term (e_tuple2 (e_option e_unit) (e_list e_issue))
         refl_check_prop_validity NRE.e_env NRE.e_term NBET.(e_tuple2 (NBET.e_option NBET.e_unit) (e_list e_issue));
 
+      mk_tac_step_2 0 "check_type_erasable"
+        refl_check_type_erasable RE.e_env RE.e_term (e_tuple2 (e_option e_unit) (e_list e_issue))
+        refl_check_type_erasable NRE.e_env NRE.e_term NBET.(e_tuple2 (NBET.e_option NBET.e_unit) (e_list e_issue));
+
       mk_tac_step_4 0 "check_match_complete"
         refl_check_match_complete RE.e_env RE.e_term RE.e_term (e_list RE.e_pattern)
                 (e_option (e_tuple2 (e_list RE.e_pattern) (e_list (e_list RE.e_binding))))
